test/Number.v
@@ -1,7 +1,7 @@
 From Parsec Require Import
      Number.
 
-Goal parse (liftA2 pair parseDec parseHex) "23Fa0$" = inr (23, 4000)%N.
+Goal parse (liftA2 pair parseDec parseHex) "23Fa0$" = inr (23, 4000, "$")%N.
 Proof. reflexivity. Qed.
 
 Goal parse parseDec "FFF" = inl (Some "Not a decimal number.").
