test/Token.v
@@ -9,7 +9,7 @@ Definition istchar (a : ascii) : bool :=
 Definition parseToken : parser string :=
   string_of_list_ascii <$> many1 (satisfy istchar).
 
-Goal parse parseToken "GET / HTTP/1.1" = inr "GET".
+Goal parse parseToken "GET / HTTP/1.1" = inr ("GET", " / HTTP/1.1").
 Proof. reflexivity. Qed.
 
 (** https://www.rfc-editor.org/rfc/rfc3986.html#section-2.1 *)
@@ -17,13 +17,13 @@ Definition parsePctEncoded : parser string :=
   liftA2 String (expect "%"%char)
          (string_of_list_ascii <$> manyN 2 (satisfy ishexdig)).
 
-Goal parse parsePctEncoded "%123" = inr "%12".
+Goal parse parsePctEncoded "%123" = inr ("%12", "3").
 Proof. reflexivity. Qed.
 
-Goal string_of_list_ascii <$>
-     parse (manyN 3 (satisfy isdigit)) "412404 Not Found" = inr "412".
+Goal parse (string_of_list_ascii <$> manyN 3 (satisfy isdigit))
+     "412404 Not Found" = inr ("412", "404 Not Found").
 Proof. reflexivity. Qed.
 
-Goal string_of_list_ascii <$>
-     parse (manyN 3 (satisfy isdigit)) "40" = inl None.
+Goal parse (string_of_list_ascii <$> manyN 3 (satisfy isdigit))
+     "40" = inl None.
 Proof. reflexivity. Qed.
